More about arrays: aloc are now per cell, loc_array is a union, WIP to prove modifies for upd

ulib/LowStar.Permissions.Array.fst
@@ -6,6 +6,7 @@ open FStar.HyperStack.ST
 module F = FStar.FunctionalExtensionality
 module G = FStar.Ghost
 module U32 = FStar.UInt32
+module MG = FStar.ModifiesGen
 
 open LowStar.Permissions
 open LowStar.Permissions.References
@@ -18,28 +19,30 @@ noeq type array (a:Type0) :Type0 =
     content:HST.reference (Seq.lseq (value_with_perms a) (U32.v max_length)) ->
     idx:U32.t ->
     length:U32.t{U32.v idx + U32.v length <= U32.v max_length} ->
-    b_pid:perm_id ->
+    pid:perm_id ->
     array a
 
-let length (#a:Type) (b:array a) = UInt32.v b.length
+(*** Definitions of Ghost operations and predicates on arrays ***)
 
-let get (#a:Type) (h:HS.mem) (b:array a) (i:nat{i < length b}) =
+let length (#a:Type) (b:array a) : nat = UInt32.v b.length
+
+let get (#a:Type) (h:HS.mem) (b:array a) (i:nat{i < length b}) : GTot a =
   let ( _, perm_map ) = Seq.index (HS.sel h b.content) (U32.v b.idx + i) in
-  get_snapshot_from_pid (Ghost.reveal perm_map) b.b_pid
+  get_snapshot_from_pid (Ghost.reveal perm_map) b.pid
 
-let live_cell (#a:Type) (h:HS.mem) (b:array a) (i:nat{i < length b}) =
+let live_cell (#a:Type) (h:HS.mem) (b:array a) (i:nat{i < length b}) : Type0 =
   let (_, perm_map) = Seq.index (HS.sel h b.content) (U32.v b.idx + i) in
-  get_permission_from_pid (Ghost.reveal perm_map) b.b_pid >. 0.0R
+  get_permission_from_pid (Ghost.reveal perm_map) b.pid >. 0.0R /\ HS.contains h b.content
 
-let live (#a:Type) (h:HS.mem) (b:array a) =
+let live (#a:Type) (h:HS.mem) (b:array a) : Type0 =
   HS.contains h b.content /\
   (forall (i:nat{i < length b}). {:pattern (get h b i)} live_cell h b i)
 
-let writeable_cell (#a:Type) (h:HS.mem) (b:array a) (i:nat{i < length b}) =
+let writeable_cell (#a:Type) (h:HS.mem) (b:array a) (i:nat{i < length b}) : Type0 =
   let (_, perm_map) = Seq.index (HS.sel h b.content) (U32.v b.idx + i) in
-  get_permission_from_pid (Ghost.reveal perm_map) b.b_pid == 1.0R
+  get_permission_from_pid (Ghost.reveal perm_map) b.pid == 1.0R /\ HS.contains h b.content
 
-let writeable (#a:Type) (h:HS.mem) (b:array a) =
+let writeable (#a:Type) (h:HS.mem) (b:array a) : Type0 =
   HS.contains h b.content /\
   (forall (i:nat{i < length b}). writeable_cell h b i)
 
@@ -47,6 +50,119 @@ let lemma_writeable_implies_live (#a:Type) (h:HS.mem) (b:array a)
   : Lemma (requires writeable h b)
           (ensures live h b)
    = ()
+
+let as_seq (#a:Type) (h:HS.mem) (b:array a) : GTot (s:Seq.seq a{Seq.length s == length b}) =
+  let s = HS.sel h b.content in
+  Seq.init (length b) (fun x -> fst (Seq.index s (U32.v b.idx + x))) 
+
+let equiv_get_as_seq (#a:Type) (h:HS.mem) (b:array a) (i:nat{i < length b /\ live_cell h b i})
+  : Lemma (Seq.index (as_seq h b) i == get h b i)
+  = ()
+
+let sel (#a: Type0)  (h: HS.mem) (b: array a) (i:nat{i < length b}) : GTot (with_perm a) =
+  let (_, perm_map) = Seq.index (HS.sel h b.content) (U32.v b.idx + i) in
+  let perm = get_permission_from_pid (Ghost.reveal perm_map) b.pid in
+  let snapshot = get_snapshot_from_pid (Ghost.reveal perm_map) b.pid in
+  { wp_v = snapshot; wp_perm = perm}
+
+(*** Definitions of locations for arrays with permissions ***)
+
+// We need to define the atomic locations cell per cell. We will then define loc_buffer as the union of aloc of cells
+// The reason for this is that we want to prove that the loc of the union of two buffers corresponds to the union of locs
+// of the two smaller buffers.
+noeq
+type ucell_ : Type0 = {
+  b_index:nat;
+  b_pid:perm_id;
+}
+
+val ucell (region:HS.rid) (addr:nat) : Tot Type0
+let ucell region addr = ucell_
+
+let frameOf (#a:Type0) (b:array a) : Tot HS.rid = HS.frameOf b.content
+let as_addr (#a:Type0) (b:array a) : GTot nat = HS.as_addr b.content
+
+// let uarray_of_array (#a:Type0) (b:array a) : Tot (uarray (frameOf b) (as_addr b)) =
+//   { b_max_length = U32.v b.max_length;
+//     b_offset = U32.v b.idx;
+//     b_length = U32.v b.length;
+//     b_pid = b.pid }
+
+let ucell_preserved (#r:HS.rid) (#a:nat) (b:ucell r a) (h0 h1:HS.mem) : GTot Type0 =
+  forall (t:Type0) (b':array t).
+    (frameOf b' == r /\ as_addr b' == a /\ b'.pid == b.b_pid /\
+      b.b_index >= U32.v b'.idx /\ b.b_index < U32.v b'.idx + U32.v b'.length ==> // If this cell is part of the buffer
+        (let i = b.b_index - U32.v b'.idx in // This cell corresponds to index i in the buffer
+         (live_cell h0 b' i ==> live_cell h1 b' i) /\ // If this cell is preserved, then its liveness is preserved
+         (sel h0 b' i == sel h1 b' i))) // And its contents (snapshot + permission) are the same
+
+// Two cells are included if they are equal: Same pid and same index in the buffer
+let ucell_includes (#r: HS.rid) (#a: nat) (c1 c2: ucell r a) : GTot Type0 =
+  c1.b_pid == c2.b_pid /\
+  c1.b_index == c2.b_index
+  
+
+let ucell_disjoint (#r:HS.rid) (#a:nat) (c1 c2:ucell r a) : GTot Type0 =
+  c1.b_index <> c2.b_index \/           // Either the cells are different (i.e. spatially disjoint)
+  c1.b_pid <> c2.b_pid                 // Or they don't have the same permission
+
+let cls : MG.cls ucell = MG.Cls #ucell
+  ucell_includes
+  (fun #r #a x -> ())
+  (fun #r #a x1 x2 x3 -> ())
+  ucell_disjoint
+  (fun #r #a x1 x2 -> ())
+  (fun #r #a larger1 larger2 smaller1 smaller2 -> ())
+  ucell_preserved
+  (fun #r #a x h -> ())
+  (fun #r #a x h1 h2 h3 -> ())
+  (fun #r #a b h1 h2 f -> admit())
+
+let bloc = MG.loc cls
+
+let loc_union (l1 l2:bloc) = MG.loc_union #ucell #cls l1 l2
+let loc_disjoint (l1 l2:bloc) = MG.loc_disjoint #ucell #cls l1 l2
+let loc_includes (l1 l2:bloc) = MG.loc_includes #ucell #cls l1 l2
+
+let loc_cell (#a:Type) (b:array a) (i:nat{i < length b}) : GTot bloc =
+  let r = frameOf b in
+  let a = as_addr b in
+  let aloc = {
+    b_index = U32.v b.idx + i;       // The index of the cell is the index inside the bigger array
+    b_pid = b.pid;
+  } in
+  MG.loc_of_aloc #ucell #cls #r #a aloc
+
+// The location of an array is the recursive union of all of its cells
+let rec compute_loc_array (#a:Type) (b:array a) (i:nat{i <= length b}) 
+  : GTot bloc
+  (decreases (length b - i))
+  = if i = length b then MG.loc_none
+    else loc_cell b i `MG.loc_union #ucell #cls` compute_loc_array b (i+1)
+
+let loc_array (#a:Type) (b:array a) : GTot bloc =
+  compute_loc_array b 0
+
+// The location of a cell of the array is included in the global loc_array
+let lemma_includes_loc_cell_loc_array (#a:Type) (b:array a) (i:nat{i < length b})
+  : Lemma (loc_includes (loc_array b) (loc_cell b i))
+  =
+  let rec aux (j:nat{j <= i}) : Lemma 
+    (ensures loc_includes (compute_loc_array b j) (loc_cell b i))
+    (decreases (i - j))
+    =
+    if j = i then begin
+      MG.loc_includes_refl #ucell #cls (loc_cell b i);
+      MG.loc_includes_union_l #ucell #cls (loc_cell b i) (compute_loc_array b (j+1)) (loc_cell b i)
+    end else begin
+      aux (j+1);
+      MG.loc_includes_union_l #ucell #cls (loc_cell b j) (compute_loc_array b (j+1)) (loc_cell b i)
+    end
+  in aux 0
+  
+let modifies (s:bloc) (h0 h1:HS.mem) : GTot Type0 = MG.modifies s h0 h1
+
+(*** Stateful operations implementing the ghost specifications ***)
 
 val index (#a:Type) (b:array a) (i:UInt32.t{UInt32.v i < length b})
   : Stack a (requires fun h -> live h b)
@@ -58,18 +174,12 @@ let index #a b i =
   let ( v, _ ) = Seq.index s (U32.v b.idx + U32.v i) in
   v
 
-let as_seq (#a:Type) (h:HS.mem) (b:array a) : GTot (s:Seq.seq a{Seq.length s == length b}) =
-  let s = HS.sel h b.content in
-  Seq.init (length b) (fun x -> fst (Seq.index s (U32.v b.idx + x))) 
-
-let equiv_get_as_seq (#a:Type) (h:HS.mem) (b:array a) (i:nat{i < length b /\ live_cell h b i})
-  : Lemma (Seq.index (as_seq h b) i == get h b i)
-  = ()
 
 //TODO: Need to add modifies. First need to define locs
 val upd (#a:Type) (b:array a) (i:UInt32.t{UInt32.v i < length b}) (v:a)
     : Stack unit (requires fun h -> writeable h b)
                  (ensures fun h0 _ h1 ->  writeable h1 b /\
+                                       modifies (loc_array b) h0 h1 /\
                                        as_seq h1 b == Seq.upd (as_seq h0 b) (U32.v i) v)
 
 let upd #a b i v =
@@ -79,11 +189,40 @@ let upd #a b i v =
   let sb0 = Seq.slice s (U32.v b.idx) (U32.v b.idx + U32.v b.length) in
   let (v_init, perm_map) = Seq.index s (U32.v b.idx + U32.v i) in
   assert (writeable_cell h0 b (U32.v i));
-  let sb1 = Seq.upd sb0 (U32.v i) (v, Ghost.hide (change_snapshot #a #v_init (Ghost.reveal perm_map) b.b_pid v)) in
+  let sb1 = Seq.upd sb0 (U32.v i) (v, Ghost.hide (change_snapshot #a #v_init (Ghost.reveal perm_map) b.pid v)) in
   let s1 = Seq.replace_subseq s (U32.v b.idx) (U32.v b.idx + U32.v b.length) sb1 in
   b.content := s1;
   let h1 = get() in
-  assert (as_seq h1 b `Seq.equal` Seq.upd (as_seq h0 b) (U32.v i) v)
+  assert (as_seq h1 b `Seq.equal` Seq.upd (as_seq h0 b) (U32.v i) v);
+  let r = frameOf b in
+  let n = as_addr b in
+  // MG.modifies_intro (loc_cell b (U32.v i)) h0 h1
+  //   (fun r -> ())
+  //   (fun t pre p -> ())// modifies_mrefs_disjoint b h0 h1 t pre p)
+  //   (fun t pre p -> ())
+  //   (fun r n -> ())
+  //   (fun r' a' b' -> admit())
+  
+  
+  MG.modifies_aloc_intro
+    #ucell #cls
+    #r #n
+    ({b_index = U32.v b.idx + U32.v i; b_pid = b.pid})
+    h0 h1
+    (fun r -> ())
+    (fun t pre b -> ())
+    (fun t pre b -> ())
+    (fun r n -> ())
+    (fun aloc' -> 
+      let aloc = ({b_index = U32.v b.idx + U32.v i; b_pid = b.pid}) in
+      assert (ucell_disjoint aloc aloc');
+      admit();
+      if aloc.b_index <> aloc'.b_index then ()
+      else
+      admit());
+  assert (modifies (loc_cell b (U32.v i)) h0 h1);
+  lemma_includes_loc_cell_loc_array b (U32.v i);
+  MG.modifies_loc_includes (loc_array b) h0 h1 (loc_cell b (U32.v i))
 
 val gsub (#a:Type0) (b:array a) (i:U32.t) (len:U32.t)
   :Ghost (array a)
